Attempts at closure only with one box

theories/Syntax/iS4_Syntax.v
@@ -142,6 +142,8 @@ Definition ClosSubform Γ : Ensemble form := fun φ => exists ψ, In _ Γ ψ /\ 
 
 Definition Clos Γ : Ensemble form := ClosOneTwoBox (ClosSubform Γ).
 
+Definition Clos' Γ : Ensemble form := ClosOneBox (ClosSubform Γ).
+
 Lemma Incl_Set_ClosSubform : forall Γ, Included _ Γ (ClosSubform Γ).
 Proof.
 intros Γ φ Hφ. unfold In. exists φ ; split ; auto. destruct φ ; simpl ; auto.
@@ -233,6 +235,49 @@ unfold ClosSubform in *. destruct Hφ. destruct H. unfold In in H. inversion H.
        apply subform_trans with (φ:=Box (Box x0)) ; auto. simpl ; auto. }
 Qed.
 
+Lemma Incl_ClosSubform_Clos' : forall Γ, Included _ (ClosSubform (Clos' Γ)) (Clos' Γ).
+Proof.
+intros Γ φ Hφ. unfold In in *. unfold Clos' in *. unfold ClosOneBox in *.
+unfold ClosSubform in *. destruct Hφ. destruct H. unfold In in H. inversion H.
+- subst. inversion H1. destruct H2. apply Union_introl. unfold In. exists x0. split ; auto.
+  apply subform_trans with (φ:=x) ; auto.
+- subst. unfold In in H1. inversion H1 ; subst.
+  unfold In in H2. destruct H2. destruct H2 ; subst. destruct H2.
+  destruct x0 ; simpl in * ; destruct H0 ; auto.
+  apply Union_intror. unfold In. exists (# n).
+  split ; auto. exists x1 ; auto. destruct H0 ; subst.
+  apply Union_introl. unfold In. exists x1 ; auto. inversion H0.
+  apply Union_intror. unfold In. exists Bot.
+  split ; auto. exists x1 ; auto. destruct H0 ; subst.
+  apply Union_introl. unfold In. exists x1 ; auto. inversion H0.
+  apply Union_intror. unfold In. exists (x0_1 ∧ x0_2).
+  split ; auto. exists x1 ; auto. destruct H0 ; subst.
+  apply Union_introl. unfold In. exists x1 ; auto.
+  apply Union_introl. unfold In. exists x1 ; split ; auto.
+  apply subform_trans with (φ:=x0_1 ∧ x0_2) ; auto. simpl ; auto.
+  apply Union_intror. unfold In. exists (x0_1 ∨ x0_2).
+  split ; auto. exists x1 ; auto. destruct H0 ; subst.
+  apply Union_introl. unfold In. exists x1 ; auto.
+  apply Union_introl. unfold In. exists x1 ; split ; auto.
+  apply subform_trans with (φ:=x0_1 ∨ x0_2) ; auto. simpl ; auto.
+  apply Union_intror. unfold In. exists (x0_1 --> x0_2).
+  split ; auto. exists x1 ; auto. destruct H0 ; subst.
+  apply Union_introl. unfold In. exists x1 ; auto.
+  apply Union_introl. unfold In. exists x1 ; split ; auto.
+  apply subform_trans with (φ:=x0_1 --> x0_2) ; auto. simpl ; auto.
+  apply Union_intror. unfold In. exists (Box x0).
+  split ; auto. exists x1 ; auto.
+  apply Union_introl. unfold In. exists x1 ; split ; auto.
+ apply subform_trans with (φ:=Box x0) ; auto. simpl ; auto.
+Qed.
+
+Lemma Box_UnBox_BoxOne_id : forall l, map Box (map UnBox (map BoxOne l)) = map BoxOne l.
+Proof.
+induction l ; simpl ; intuition.
+destruct a ; simpl ; subst ; auto. 1-5: rewrite IHl ; auto.
+destruct a ; simpl ; auto. 1-6: rewrite IHl ; auto.
+Qed.
+
 Lemma Box_UnBox_BoxTwo_id : forall l, map Box (map UnBox (map BoxTwo l)) = map BoxTwo l.
 Proof.
 induction l ; simpl ; intuition.
@@ -251,6 +296,11 @@ induction φ ; simpl ; auto.
 destruct φ ; simpl ; auto.
 Qed.
 
+Lemma BoxOne_UnBox_fixpoint : forall φ, BoxOne φ = Box (UnBox (BoxOne φ)).
+Proof.
+induction φ ; simpl ; auto.
+Qed.
+
 Lemma BoxTwo_UnBox_fixpoint : forall φ, BoxTwo φ = Box (UnBox (BoxTwo φ)).
 Proof.
 induction φ ; simpl ; auto.
@@ -265,6 +315,12 @@ destruct H0 ; subst. exfalso ; apply H. exists (Box (UnBox (UnBox x0))).
 apply UnBox_BoxTwo.
 Qed.
 
+Lemma In_Clos'_not_box : forall Γ φ, ((exists ψ, φ = Box ψ) -> False) -> (Clos' Γ) φ -> (ClosSubform Γ) φ.
+Proof.
+intros. destruct H0 ; auto. destruct H0 ; auto. destruct H0. destruct H0 ; subst.
+exfalso. apply H. exists (UnBox x0). apply UnBox_BoxOne.
+Qed.
+
 Lemma In_Clos_BoxTwo : forall Γ φ, (Clos Γ) φ -> (Clos Γ) (BoxTwo φ).
 Proof.
 induction φ.
@@ -277,6 +333,14 @@ exists (Box Bot). simpl ; split ; auto.
 exists (Box (φ1 ∧ φ2)). simpl ; split ; auto.
 exists (Box (φ1 ∨ φ2)). simpl ; split ; auto.
 exists (Box (φ1 --> φ2)). simpl ; split ; auto.
+Qed.
+
+Lemma In_Clos'_BoxOne : forall Γ φ, (Clos' Γ) φ -> (Clos' Γ) (BoxOne φ).
+Proof.
+induction φ.
+1-5: intros ; apply Union_intror ; eexists ; split ; auto ; apply In_Clos'_not_box ; auto.
+1-5: intro H0 ; destruct H0 ; inversion H0.
+intros. destruct φ ; simpl in * ; auto.
 Qed.
 
 
