theories/GHC/iS4_Lindenbaum_lem.v
@@ -386,6 +386,119 @@ remember (form_index a) as n. destruct n ; simpl.
      inversion H4 ; subst. 2: inversion H5. apply Id. apply IdRule_I ; auto.
 Qed.
 
+Lemma restr_quasi_prime_Lind_theory': forall Γ Δ ψ,
+  Included _ Δ (Clos' Γ) ->
+  ~ iS4H_prv (Δ, ψ) ->
+  restr_quasi_prime (Clos' Γ) (Lind_theory (Clos' Γ) Δ ψ).
+Proof.
+intros Γ Δ ψ Incl H0 a b Horg Hor H1. remember (Clos' Γ) as CΓ.
+
+apply H1. left. exists (form_index a).
+remember (form_index a) as n. destruct n ; simpl.
+- unfold choice_code. unfold choice_form. unfold In.
+  right. repeat split. 3: rewrite Heqn ; apply form_enum_index.
+  subst. apply Incl_ClosSubform_Clos'. exists (a ∨ b). split ; auto.
+  simpl. right ; apply in_or_app ; left ; destruct a ; simpl ; auto.
+  intro. apply H1. right. exists (form_index b).
+  remember (form_index b) as m. destruct m ; simpl.
+  + rewrite Heqm in Heqn. apply form_index_inj in Heqn.
+     subst. exfalso.
+     pose (Under_Lind_theory (Clos' Γ) Δ ψ Incl H0). apply n.
+    apply MP with (ps:=[(Lind_theory (Clos' Γ) Δ ψ, (Or a a) --> ψ);
+    (Lind_theory (Clos' Γ) Δ ψ, (Or a a))]). 2: apply MPRule_I. intros. inversion H2 ; subst.
+    apply MP with (ps:=[(Lind_theory (Clos' Γ) Δ ψ, (a --> ψ) --> (Or a a --> ψ));
+    (Lind_theory (Clos' Γ) Δ ψ, (a --> ψ))]). 2: apply MPRule_I. intros. inversion H3 ; subst.
+    apply MP with (ps:=[(Lind_theory (Clos' Γ) Δ ψ, (a --> ψ) --> (a --> ψ) --> (Or a a --> ψ));
+    (Lind_theory (Clos' Γ) Δ ψ, (a --> ψ))]). 2: apply MPRule_I. intros. inversion H4 ; subst.
+    apply Ax. apply AxRule_I. left. apply IA5_I. exists a. exists a. exists ψ. auto.
+    inversion H5 ; subst. 2: inversion H6.
+    apply iS4H_Deduction_Theorem with (s:=(Union (form) (Lind_theory (Clos' Γ) Δ ψ) (Singleton (form) a), ψ)) ; auto.
+    apply iS4H_monot with (Γ1:=Union form (Lind_theory (Clos' Γ) Δ ψ) (Singleton form a)) in H ; auto.
+    simpl ; intros c Hc. inversion Hc ; subst. apply Union_introl. apply Lind_theory_extens ; auto.
+    inversion H6 ; subst ; apply Union_intror ; apply In_singleton.
+    inversion H4 ; subst. 2: inversion H5.
+    apply iS4H_Deduction_Theorem with (s:=(Union (form) (Lind_theory (Clos' Γ) Δ ψ) (Singleton (form) a), ψ)) ; auto.
+    apply iS4H_monot with (Γ1:=Union form (Lind_theory (Clos' Γ) Δ ψ) (Singleton form a)) in H ; auto.
+    simpl ; intros c Hc. inversion Hc ; subst. apply Union_introl. apply Lind_theory_extens ; auto.
+    inversion H5 ; subst ; apply Union_intror ; apply In_singleton.
+    inversion H3 ; subst. 2: inversion H4. apply Id. apply IdRule_I ; auto.
+  + subst. unfold choice_code. unfold choice_form. unfold In. right. repeat split.
+     subst. apply Incl_ClosSubform_Clos'. exists (a ∨ b). split ; auto.
+     simpl. right ; apply in_or_app ; right ; destruct b ; simpl ; auto.
+     2: rewrite Heqm ; apply form_enum_index. intro.
+     pose (Under_Lind_theory (Clos' Γ) Δ ψ Incl H0). apply n.
+     apply MP with (ps:=[(Lind_theory (Clos' Γ) Δ ψ, (Or a b) --> ψ);
+     (Lind_theory (Clos' Γ) Δ ψ, (Or a b))]). 2: apply MPRule_I. intros. inversion H3 ; subst.
+     apply MP with (ps:=[(Lind_theory (Clos' Γ) Δ ψ, (b --> ψ) --> (Or a b --> ψ));
+     (Lind_theory (Clos' Γ) Δ ψ, (b --> ψ))]). 2: apply MPRule_I. intros. inversion H4 ; subst.
+     apply MP with (ps:=[(Lind_theory (Clos' Γ) Δ ψ, (a --> ψ) --> (b --> ψ) --> (Or a b --> ψ));
+     (Lind_theory (Clos' Γ) Δ ψ, (a --> ψ))]). 2: apply MPRule_I. intros. inversion H5 ; subst.
+     apply Ax. apply AxRule_I. left. apply IA5_I. exists a. exists b. exists ψ. auto.
+     inversion H6 ; subst. 2: inversion H7.
+     apply iS4H_Deduction_Theorem with (s:=(Union (form) (Lind_theory (Clos' Γ) Δ ψ) (Singleton (form) a), ψ)) ; auto.
+     apply iS4H_monot with (Γ1:=Union form (Lind_theory (Clos' Γ) Δ ψ) (Singleton form a)) in H ; auto.
+     simpl ; intros c Hc. inversion Hc ; subst. apply Union_introl. apply Lind_theory_extens ; auto.
+     inversion H7 ; subst ; apply Union_intror ; apply In_singleton.
+     inversion H5 ; subst. 2: inversion H6.
+     apply iS4H_Deduction_Theorem with (s:=(Union (form) (Lind_theory (Clos' Γ) Δ ψ) (Singleton (form) b), ψ)) ; auto.
+     apply iS4H_monot with (Γ1:=Union form (Lind_theory (Clos' Γ) Δ ψ) (Singleton form b)) in H2 ; auto.
+     simpl ; intros c Hc. inversion Hc ; subst. apply Union_introl. unfold In. exists m ; auto.
+     inversion H6 ; subst ; apply Union_intror ; apply In_singleton.
+     inversion H4 ; subst. 2: inversion H5. apply Id. apply IdRule_I ; auto.
+- unfold choice_code. unfold choice_form. unfold In.
+  right. repeat split. 3: rewrite Heqn ; apply form_enum_index.
+  subst. apply Incl_ClosSubform_Clos'. exists (a ∨ b). split ; auto.
+  simpl. right ; apply in_or_app ; left ; destruct a ; simpl ; auto.
+  intro. apply H1. right. exists (form_index b).
+  remember (form_index b) as m. destruct m ; simpl.
+  + subst. unfold choice_code. unfold choice_form. unfold In. right. repeat split.
+     subst. apply Incl_ClosSubform_Clos'. exists (a ∨ b). split ; auto.
+     simpl. right ; apply in_or_app ; right ; destruct b ; simpl ; auto.
+     2: rewrite Heqm ; apply form_enum_index. intro.
+     pose (Under_Lind_theory (Clos' Γ) Δ ψ Incl H0). apply n0.
+     apply MP with (ps:=[(Lind_theory (Clos' Γ) Δ ψ, (Or a b) --> ψ);
+     (Lind_theory (Clos' Γ) Δ ψ, (Or a b))]). 2: apply MPRule_I. intros. inversion H3 ; subst.
+     apply MP with (ps:=[(Lind_theory (Clos' Γ) Δ ψ, (b --> ψ) --> (Or a b --> ψ));
+     (Lind_theory (Clos' Γ) Δ ψ, (b --> ψ))]). 2: apply MPRule_I. intros. inversion H4 ; subst.
+     apply MP with (ps:=[(Lind_theory (Clos' Γ) Δ ψ, (a --> ψ) --> (b --> ψ) --> (Or a b --> ψ));
+     (Lind_theory (Clos' Γ) Δ ψ, (a --> ψ))]). 2: apply MPRule_I. intros. inversion H5 ; subst.
+     apply Ax. apply AxRule_I. left. apply IA5_I. exists a. exists b. exists ψ. auto.
+     inversion H6 ; subst. 2: inversion H7.
+     apply iS4H_Deduction_Theorem with (s:=(Union (form) (Lind_theory (Clos' Γ) Δ ψ) (Singleton (form) a), ψ)) ; auto.
+     apply iS4H_monot with (Γ1:=Union form (Lind_theory (Clos' Γ) Δ ψ) (Singleton form a)) in H ; auto.
+     simpl ; intros c Hc. inversion Hc ; subst. apply Union_introl. unfold In ; exists n ; auto.
+     inversion H7 ; subst ; apply Union_intror ; apply In_singleton.
+     inversion H5 ; subst. 2: inversion H6.
+     apply iS4H_Deduction_Theorem with (s:=(Union (form) (Lind_theory (Clos' Γ) Δ ψ) (Singleton (form) b), ψ)) ; auto.
+     apply iS4H_monot with (Γ1:=Union form (Lind_theory (Clos' Γ) Δ ψ) (Singleton form b)) in H2 ; auto.
+     simpl ; intros c Hc. inversion Hc ; subst. apply Union_introl. apply Lind_theory_extens ; auto.
+     inversion H6 ; subst ; apply Union_intror ; apply In_singleton.
+     inversion H4 ; subst. 2: inversion H5. apply Id. apply IdRule_I ; auto.
+  + subst. unfold choice_code. unfold choice_form. unfold In. right. repeat split.
+     subst. apply Incl_ClosSubform_Clos'. exists (a ∨ b). split ; auto.
+     simpl. right ; apply in_or_app ; right ; destruct b ; simpl ; auto.
+     2: rewrite Heqm ; apply form_enum_index. intro.
+     pose (Under_Lind_theory (Clos' Γ) Δ ψ Incl H0). apply n0.
+     apply MP with (ps:=[(Lind_theory (Clos' Γ) Δ ψ, (Or a b) --> ψ);
+     (Lind_theory (Clos' Γ) Δ ψ, (Or a b))]). 2: apply MPRule_I. intros. inversion H3 ; subst.
+     apply MP with (ps:=[(Lind_theory (Clos' Γ) Δ ψ, (b --> ψ) --> (Or a b --> ψ));
+     (Lind_theory (Clos' Γ) Δ ψ, (b --> ψ))]). 2: apply MPRule_I. intros. inversion H4 ; subst.
+     apply MP with (ps:=[(Lind_theory (Clos' Γ) Δ ψ, (a --> ψ) --> (b --> ψ) --> (Or a b --> ψ));
+     (Lind_theory (Clos' Γ) Δ ψ, (a --> ψ))]). 2: apply MPRule_I. intros. inversion H5 ; subst.
+     apply Ax. apply AxRule_I. left. apply IA5_I. exists a. exists b. exists ψ. auto.
+     inversion H6 ; subst. 2: inversion H7.
+     apply iS4H_Deduction_Theorem with (s:=(Union (form) (Lind_theory (Clos' Γ) Δ ψ) (Singleton (form) a), ψ)) ; auto.
+     apply iS4H_monot with (Γ1:=Union form (Lind_theory (Clos' Γ) Δ ψ) (Singleton form a)) in H ; auto.
+     simpl ; intros c Hc. inversion Hc ; subst. apply Union_introl. unfold In. exists n ; auto.
+     inversion H7 ; subst ; apply Union_intror ; apply In_singleton.
+     inversion H5 ; subst. 2: inversion H6.
+     apply iS4H_Deduction_Theorem with (s:=(Union (form) (Lind_theory (Clos' Γ) Δ ψ) (Singleton (form) b), ψ)) ; auto.
+     apply iS4H_monot with (Γ1:=Union form (Lind_theory (Clos' Γ) Δ ψ) (Singleton form b)) in H2 ; auto.
+     simpl ; intros c Hc. inversion Hc ; subst. apply Union_introl. unfold In. exists m ; auto.
+     inversion H6 ; subst ; apply Union_intror ; apply In_singleton.
+     inversion H4 ; subst. 2: inversion H5. apply Id. apply IdRule_I ; auto.
+Qed.
+
 (* A prime pair is consistent. *)
 
 Lemma Consist_nLind_theory : forall n Γ Δ ψ,
@@ -465,6 +578,28 @@ repeat split.
 - apply stable_Lind_theory ; auto.
 - pose restr_quasi_prime_Lind_theory ; auto.
 - intro. apply Under_Lind_theory with (Γ:=(Clos Γ)) in H1 ; auto.
+Qed.
+
+Lemma Lindenbaum' Γ Δ ψ :
+  In _ (Clos' Γ) ψ ->
+  Included _ Δ (Clos' Γ) ->
+  ~ iS4H_prv (Δ, ψ) ->
+  exists Δm, Included _ Δ Δm
+           /\ Included _ Δm (Clos' Γ)
+           /\ restr_closed (Clos' Γ) Δm
+           /\ restr_stable (Clos' Γ) Δm
+           /\ restr_quasi_prime (Clos' Γ) Δm
+           /\ ~ iS4H_prv (Δm, ψ).
+Proof.
+intros.
+exists (Lind_theory (Clos' Γ) Δ ψ).
+repeat split.
+- intro. apply Lind_theory_extens.
+- apply incl_Lind_theory ; auto.
+- apply restr_closeder_Lind_theory ; auto.
+- apply stable_Lind_theory ; auto.
+- pose restr_quasi_prime_Lind_theory' ; auto.
+- intro. apply Under_Lind_theory with (Γ:=(Clos' Γ)) in H1 ; auto.
 Qed.
 
 End Lindenbaum.
